src/tls/Pkg.Tree.fst
@@ -4,6 +4,7 @@ open Mem
 open Pkg
 open Idx
 
+module M = LowStar.Modifies
 module DT = DefineTable
 
 /// We use subtrees to specify KDF usages. We hope we can erase
@@ -22,7 +23,7 @@ and children' (par_ideal:Type0) = list (label * tree' par_ideal)
 
 // would prefer to use Map.t, but positivity check fails
 
-inline_for_extraction
+inline_for_extraction noextract
 let max x y = if x <= y then y else x
 
 // induction on n-ary trees requires explicit termination
@@ -47,43 +48,220 @@ type tree (p:Type0) =
 type children (p:Type0) =
   (if model then children' p else no_tree)
 
+// Used to start building children
+inline_for_extraction noextract
+let no_children (p:Type0) : children p =
+  (if model then [] <: children' p else erased_tree)
+
 inline_for_extraction
-let rec find_lbl (#p:Type0) (u:children p) (l: label) : option (tree p) =
-  if model then
-    let u' : children' p = u in
-    match u' with
-    | [] -> None
-    | (lbl, t) :: tl ->
-      if lbl = l then Some t
-      else
-	let tl : children p = tl in
-	find_lbl tl l
-  else None
+let rec find_lbl' (#p:Type0) (u:children' p) (l: label) : option (tree' p) =
+  match u with
+  | [] -> None
+  | (lbl, t) :: tl ->
+    if lbl = l then Some t
+    else find_lbl' tl l
+
+noextract
+let rec find_lbl (#p:Type0) (u:children p) (l:label) : option (tree p) =
+  if model then find_lbl' (u <: children' p) l else None
+
+inline_for_extraction
+let has_lbl' (#p:Type0) (u:children' p) (l: label) =
+  Some? (find_lbl' u l)
 
 inline_for_extraction
 let has_lbl (#p:Type0) (u:children p) (l: label) =
-  if model then Some? (find_lbl u l) else false
+  if model then (u <: children' p) `has_lbl'` l else false
+
+noextract
+let down' (#p:Type0) (u:children' p) (l:label{u `has_lbl'` l}) : tree' p =
+  Some?.v (find_lbl' u l)
 
 noextract
 let down (#p:Type0) (u:children p) (l:label{u `has_lbl` l}) : tree p =
   Some?.v (find_lbl u l)
 
 noextract
-let child (#p:Type0) (u:children p) (l:label{model /\ u `has_lbl` l})
+let child (#p:Type0) (u:children' p) (l:label{u `has_lbl'` l})
   : pkg:t{Pkg?.ideal pkg ==> p}
   =
-  let x : tree' p = down u l in
+  let x : tree' p = down' u l in
   match x with
   | Leaf p -> p
   | Node p c -> p
 
+type initial_state (#p:Type0) (pkg:t{Pkg?.ideal pkg ==> p}) (h:mem) =
+  DT.empty (Pkg?.define_table pkg)
+
+(**** Tree invariant ****)
+
 (*
-let rec index_consistent (#p:Type0) (u:children p)
-  (#it:eqtype) (#vt:it->Type) (t:DT.dt vt) (h:mem) =
-  if model then
-    let u' : children' p = u in
-    match u with
-    | [] -> True
-    | (lbl,t) :: tl -> True
-  else True
+
+The structure of indexes defined in each package of the tree
+follows the structure of the tree itself:
+
+      KDF   package invariant = children invariant of usage
+     / | \
+    a  b  c   derivation labels
+   /   |   \
+[ X    Y    Z ] children (KDF usage)
+           / \
+
+if (x i) is an instance of package X, then i must be of the
+form Derive j a ctx where j is defined in KDF.
+
+Furthermore, the invariant of a node pacakge implies the
+invariant of every descendent package.
 *)
+
+let regid : eqtype = i:ii.t{ii.registered i}
+
+val tree_inv': #p:Type0 -> t:tree' p -> mem ->
+  Ghost Type0 (requires model) (ensures fun _ -> True) (decreases %[t])
+val children_inv': #vt:(regid->Type) -> DT.dt vt -> #p:Type0 -> u:children' p -> mem ->
+  Ghost Type0 (requires model) (ensures fun _ -> True) (decreases %[u])
+
+let child_instance_inv (#vt:regid->Type) (parent_dt:DT.dt vt)
+  (lbl:label) (#kt:regid->Type) (#i:regid) (k:kt i) (h:mem)
+  : Ghost Type0 (requires model) (ensures fun _ -> True) =
+  let i : pre_id = i in
+  match i  with
+  | Preshared _ _ -> False
+  | Derive j lbl' ctx -> lbl == lbl' /\
+    registered j /\ DT.defined parent_dt j
+
+let rec tree_inv' #p t h =
+  match t with
+  | Leaf p -> Pkg?.package_invariant p h
+  | Node p u -> Pkg?.package_invariant p h /\
+    children_inv' p.define_table u h
+
+and children_inv' #vt parent_dt #p u h =
+  match u with
+  | [] -> True
+  | (lbl,x)::tl ->
+    let pkg = match x with Leaf p -> p | Node p _ -> p in
+    tree_inv' x h /\ children_inv' parent_dt tl h /\
+    M.loc_disjoint (DT.loc parent_dt) (DT.loc pkg.define_table) /\
+    DT.dt_forall pkg.define_table (child_instance_inv parent_dt lbl) h
+
+let tree_inv (#p:Type0) (t:tree p) (h:mem) =
+  (if model then tree_inv' (t <: tree' p) h else True)
+
+let children_inv #vt (dt:DT.dt vt) (#p:Type0) (t:children p) (h:mem) =
+  (if model then children_inv' dt (t <: children' p) h else True)
+
+noextract
+let rec labels_of_id (i:pre_id) (acc:list label) =
+  match i with
+  | Preshared a pski -> acc
+  | Derive i l ctx -> labels_of_id i (l::acc)
+
+(*
+let x : label = assume false; "x"
+let y : label = assume false; "y"
+let _ = assert_norm (labels_of_id (Derive(Derive (Preshared Hashing.Spec.SHA1 0) x Extract) y Extract) [] == [x; y])
+*)
+
+let rec subtree (#p:Type0) (t:tree' p)
+  (#q:Type0) (c:children' q) (l:list label)
+  : Pure Type (requires model) (ensures fun _ -> True) (decreases %[l])
+  =
+  Node? t /\
+  (match l with
+  | [] -> q == Pkg?.ideal (Node?.node t) /\ Node?.children t == c
+  | lbl::tl ->
+    let c' = Node?.children t in
+    c' `has_lbl'` lbl /\
+    subtree (down' c' lbl) c tl)
+
+let rec defined_path (#p:Type0) (t:tree' p) (l:list label)
+  : GTot Type (decreases %[l]) =
+  match t with
+  | Leaf _ -> l == []
+  | Node p c ->
+    match l with
+    | [] -> False
+    | lbl::tl -> c `has_lbl'` lbl /\ defined_path (down' c lbl) tl
+
+let rec get_package (#p:Type0) (t:tree' p) (l:list label{defined_path t l})
+  : GTot (pkg ii) (decreases %[l]) =
+  match t with
+  | Leaf p -> p
+  | Node p c ->
+    match l with
+    | lbl :: tl -> get_package (down' c lbl) tl
+
+let rec get_usage (#p:Type0) (t:tree' p) (l:list label{defined_path t l})
+  : GTot (p:Type0 & children' p) (decreases %[l]) =
+  match t with
+  | Leaf p -> (| Pkg?.ideal p, ([] <: children' (Pkg?.ideal p)) |)
+  | Node pkg c ->
+    match l with
+    | [] -> (| p, c |)
+    | lbl :: tl -> get_usage (down' c lbl) tl
+
+let defined' (#p:Type0) (t:tree' p) (i:regid{model}) =
+  let path = labels_of_id i [] in
+  defined_path t path /\
+  (let pkg = get_package t path in
+  DT.defined pkg.define_table i)
+
+let defined (#p:Type0) (t:tree p) (i:regid) =
+  if model then defined' (t <: tree' p) i else True
+
+val lemma_derive_children:
+  #vt: (regid->Type) ->
+  dt: DT.dt vt ->
+  #p: Type0 ->
+  u: children' p ->
+  i: regid{DT.defined dt i} ->
+  lbl: label{u `has_lbl'` lbl} ->
+  ctx: context{wellformed_derive i lbl ctx /\ registered (derive i lbl ctx)} ->
+  k: Pkg?.key (child u lbl) (derive i lbl ctx) ->
+  h0:mem -> h1:mem ->
+  Lemma (requires model /\ children_inv' dt u h0 /\
+    DT.extended (child u lbl).define_table k h0 h1 /\
+    (child u lbl).package_invariant h1)
+  (ensures children_inv' dt u h1)
+  (decreases %[u])
+
+val lemma_derive_tree:
+  #p: Type0 ->
+  t: tree' p ->
+  h0:mem -> l:M.loc -> h1:mem ->
+  Lemma (requires model /\ tree_inv' t h0 /\ M.modifies l h0 h1 /\
+    M.loc_disjoint l l)
+  (ensures tree_inv' t h1)
+  (decreases %[t])
+
+(*
+// Local subtree invariant restoration
+let rec lemma_derive 
+  =
+  match u with
+  | [] -> ()
+  | (lbl', t) :: tl ->
+    if lbl = lbl' then
+     begin
+      lemma_
+     end
+    else lemma_derive dt tl i lbl ctx k h0 h1
+  
+  let rec aux
+    : Lemma ()
+    =
+    admit()
+    in
+  admit()
+*)
+
+(*
+Building the tree is quite technical because the tree
+invariant must be initialized (which requires the define
+table of the parent to be allocated before children can be
+defined.
+
+We provide stateful helper functions to help construct trees
+*)
+
